Phi_StdLib/PhiStd_Slice_a.thy
@@ -41,7 +41,7 @@ proc (nodef) map_2slice_a:
 \<medium_right_bracket> .
 
 proc memcpy_a:
-  requires \<open>(\<And>x. Semantic_Type T TY)\<close>
+  requires \<open>(\<And>x. Weak_Semantic_Type T TY)\<close>
   input  \<open>i\<^sub>a \<Ztypecolon> \<v>\<a>\<l> \<bbbS>\<p>\<t>\<r>[addr\<^sub>a:LEN\<^sub>a] TY\<heavy_comma> i\<^sub>b \<Ztypecolon> \<v>\<a>\<l> \<bbbS>\<p>\<t>\<r>[addr\<^sub>b:LEN\<^sub>b] TY\<heavy_comma> len \<Ztypecolon> \<v>\<a>\<l> \<nat>\<heavy_comma>
           l\<^sub>a \<Ztypecolon> \<m>\<e>\<m>[addr\<^sub>a] \<s>\<l>\<i>\<c>\<e>[i\<^sub>a,len] T\<heavy_comma> l\<^sub>b \<Ztypecolon> \<m>\<e>\<m>[addr\<^sub>b] \<s>\<l>\<i>\<c>\<e>[i\<^sub>b,len] T\<close>
   premises \<open>i\<^sub>a + len \<le> LEN\<^sub>a \<and> i\<^sub>b + len \<le> LEN\<^sub>b\<close>
